common/step_ok.v
@@ -1,0 +1,110 @@
+Require Export ho_proof_gen.
+
+Set Implicit Arguments.
+
+Section step_one.
+
+Variables (cfg : Type) (cstep : cfg -> cfg -> Prop).
+Definition Spec : Type := cfg -> (cfg -> Prop) -> Prop.
+
+(* Soundness *)
+CoInductive reaches (k : cfg) (P : cfg -> Prop) : Prop :=
+  (* reaches : Spec, but defining k and P as parameters
+     gives a cleaner definition and induction principle. *)
+| rdone : P k -> reaches k P
+| rstep : forall k', cstep k k' -> reaches k' P -> reaches k P.
+
+Definition sound Rules : Prop := subspec Rules reaches.
+
+Inductive step (X : Spec) (k : cfg) (P : cfg -> Prop) : Prop :=
+  (* step : Spec -> Spec *)
+| sdone : P k -> step X k P
+| sstep : forall k', cstep k k' -> X k' P -> step X k P.
+
+Lemma step_mono : mono step.
+Proof. destruct 2;econstructor(solve[eauto using step]). Qed.
+
+Lemma reaches_stable : subspec reaches (step reaches).
+Proof. destruct 1;econstructor(eassumption). Qed.
+
+CoFixpoint stable_sound Rules (Hstable : subspec Rules (step Rules)) : sound Rules :=
+  fun x P H =>
+  match Hstable _ _ H with
+    | sdone pf => rdone _ _ pf
+    | sstep k' Hstep H' =>
+        rstep Hstep (stable_sound Hstable _ _ H')
+  end.
+
+Lemma proof_by_t : forall (Rules : Spec), subspec Rules (step (t step Rules)) -> sound Rules.
+  intros. apply t_ext in H. apply stable_sound in H. revert H.
+  unfold sound, subspec. firstorder using t_id. apply step_mono. 
+Qed.
+
+Definition trans (X:Spec) : Spec := fun k P => exists Q, X k Q /\ (forall k', Q k' -> X k' P).
+
+Lemma mono_trans : mono trans.
+Proof.
+  destruct 2. inversion H0. econstructor; split. apply H. eassumption.
+  intros. apply H. apply H2. trivial.
+Qed.
+
+Lemma trans_ok_rule : forall X, subspec (trans X) (t step X).
+  apply rule_by_T. apply step_mono. apply mono_trans.
+  unfold subspec. intros. destruct H as [Q [HQ H]].
+  destruct HQ. specialize (H _ H0). revert H. apply step_mono. apply Tf_id.
+  eapply sstep;eauto. intros. apply Tf_idem. apply step_mono.
+  firstorder. apply T_id.
+  exists Q. split. eapply Tf_id;apply H1;assumption. intros.
+  specialize (H k'0 H2). apply Tf_base. apply step_mono. assumption.
+Qed.
+
+Lemma use_trans : forall A, subspec (trans (t step A)) (t step A).
+apply t_rule. firstorder. apply step_mono. apply trans_ok_rule.
+Qed.
+
+Lemma tstep: forall F, mono F -> forall A x P,
+    forall x', cstep x x' -> T step F A x' P -> T step F A x P.
+Proof.
+  intros. apply use_step. apply step_mono. assumption. eapply sstep;eassumption.
+Qed.
+
+Lemma tdone: forall F, mono F -> forall A x (P:cfg->Prop), P x -> T step F A x P.
+Proof.
+  intros. apply use_step. apply step_mono. assumption. eapply sdone;eassumption.
+Qed.
+
+Lemma ttrans: forall F, mono F -> forall A x Q P,
+    T step F A x Q -> (forall y, Q y -> T step F A y P) -> T step F A x P.
+Proof.
+  intros. apply Tf_idem. apply step_mono. assumption. apply Tf_t. assumption.
+  apply trans_ok_rule. unfold trans. exists Q.
+  split;assumption.
+Qed.
+
+(* X <= step(t X) ==> X <= gfp step *)
+(* X <= Step (T X) *)
+(* X (step A) <= step ((T X) A) ==> X <= t
+   ==> X reaches <= reaches, other stuff *)
+
+(* t_|_ = gfp step ==> t (gfp step) = t (t _|_) = t bot = gfp step *)
+
+(* F : higher order spec  *)
+(* F(A) <= step((T F) A)  *)
+(* gfp F <= reaches *)
+Lemma ok : forall F, mono F ->
+    (forall A, subspec (F A) (step (T step F A))) ->
+    (forall X, subspec X (F X) -> subspec X reaches)
+    (* == subspec (gfp F) reaches *).
+  intros.
+  assert (forall A, subspec (F A) (t step A)).
+  intros. apply rule_by_T. apply step_mono. apply H.  
+  unfold subspec;intros. apply H0 in H2. revert H2. apply step_mono.
+  unfold subspec;intros. apply Tf_idem. apply step_mono. assumption.
+  revert H2. apply T_mono. assumption. apply Tf_base. apply step_mono.
+  apply proof_by_t. intro;intros.
+  apply H1 in H3. apply H0 in H3.
+  revert H3. apply step_mono. apply T_rule_f. apply step_mono. assumption. assumption.
+Qed.
+
+End step_one.
+
